@prefix : <http://bimerr.iot.linkeddata.es/def/occupancy-profile#> .
@prefix owl: <http://www.w3.org/2002/07/owl#> .
@prefix rdf: <http://www.w3.org/1999/02/22-rdf-syntax-ns#> .
@prefix xml: <http://www.w3.org/XML/1998/namespace> .
@prefix xsd: <http://www.w3.org/2001/XMLSchema#> .
@prefix rdfs: <http://www.w3.org/2000/01/rdf-schema#> .
@base <http://bimerr.iot.linkeddata.es/def/occupancy-profile#> .

<http://bimerr.iot.linkeddata.es/def/occupancy-profile#> rdf:type owl:Ontology ;
                                                          <http://purl.org/dc/elements/1.1/creator> "María Poveda Villalón" ,
                                                                                                    "Raúl García Castro" ,
                                                                                                    "Serge Chávez Feria" ;
                                                          <http://purl.org/dc/elements/1.1/description> "The Occupancy Profile ontology has been developed to represent and define occupancy profiles in building spaces.|"@en ;
                                                          <http://purl.org/dc/elements/1.1/publisher> "http://www.oeg-upm.net/"@en ;
                                                          <http://purl.org/dc/elements/1.1/title> "Occupancy Profile ontology"@en ;
                                                          <http://purl.org/dc/terms/creator> <http://www.oeg-upm.net/> ;
                                                          <http://purl.org/dc/terms/license> "http://purl.org/NET/rdflicense/cc-by4.0"@en ;
                                                          <http://purl.org/vocab/vann/preferredNamespacePrefix> "op"@en ;
                                                          <http://purl.org/vocab/vann/preferredNamespaceUri> "http://bimerr.iot.linkeddata.es/def/occupancy-profile#" ;
                                                          owl:versionInfo "0.0.5" .

#################################################################
#    Annotation properties
#################################################################

###  http://purl.org/dc/elements/1.1/created
<http://purl.org/dc/elements/1.1/created> rdf:type owl:AnnotationProperty .


###  http://purl.org/dc/elements/1.1/creator
<http://purl.org/dc/elements/1.1/creator> rdf:type owl:AnnotationProperty .


###  http://purl.org/dc/elements/1.1/description
<http://purl.org/dc/elements/1.1/description> rdf:type owl:AnnotationProperty .


###  http://purl.org/dc/elements/1.1/publisher
<http://purl.org/dc/elements/1.1/publisher> rdf:type owl:AnnotationProperty .


###  http://purl.org/dc/elements/1.1/title
<http://purl.org/dc/elements/1.1/title> rdf:type owl:AnnotationProperty .


###  http://purl.org/dc/terms/creator
<http://purl.org/dc/terms/creator> rdf:type owl:AnnotationProperty .


###  http://purl.org/dc/terms/license
<http://purl.org/dc/terms/license> rdf:type owl:AnnotationProperty .


###  http://purl.org/dc/terms/modified
<http://purl.org/dc/terms/modified> rdf:type owl:AnnotationProperty .


###  http://purl.org/vocab/vann/preferredNamespacePrefix
<http://purl.org/vocab/vann/preferredNamespacePrefix> rdf:type owl:AnnotationProperty .


###  http://purl.org/vocab/vann/preferredNamespaceUri
<http://purl.org/vocab/vann/preferredNamespaceUri> rdf:type owl:AnnotationProperty .


#################################################################
#    Datatypes
#################################################################

###  http://www.w3.org/2001/XMLSchema#date
xsd:date rdf:type rdfs:Datatype .


###  http://www.w3.org/2001/XMLSchema#duration
xsd:duration rdf:type rdfs:Datatype .


###  http://www.w3.org/2001/XMLSchema#gMonthDay
xsd:gMonthDay rdf:type rdfs:Datatype .


###  http://www.w3.org/2001/XMLSchema#time
xsd:time rdf:type rdfs:Datatype .


#################################################################
#    Object Properties
#################################################################

###  http://bimerr.iot.linkeddata.es/def/occupancy-profile#composedOf
:composedOf rdf:type owl:ObjectProperty ;
            rdfs:domain :DriverSet ;
            rdfs:range :Driver ;
            rdfs:comment "Relationship that indicates the composition of a set of drivers."@en ;
            rdfs:label "composed of"@en .


###  http://bimerr.iot.linkeddata.es/def/occupancy-profile#definedByRange
:definedByRange rdf:type owl:ObjectProperty ,
                         owl:FunctionalProperty ;
                rdfs:domain :PhysicalNeed ;
                rdfs:range :ParameterRange ;
                rdfs:comment "Property used to describe occupant needs by defining comfort limits w.r.t. an environmental parameter."@en ;
                rdfs:label "defined by range"@en .


###  http://bimerr.iot.linkeddata.es/def/occupancy-profile#describedByFormula
:describedByFormula rdf:type owl:ObjectProperty ,
                             owl:FunctionalProperty ;
                    rdfs:domain :Interaction ;
                    rdfs:range :InteractionFormula ;
                    rdfs:comment "Property to relate an interaction with a formula describing the probability of occurance."@en ;
                    rdfs:label "described by formula"@en .


###  http://bimerr.iot.linkeddata.es/def/occupancy-profile#describesParameter
:describesParameter rdf:type owl:ObjectProperty ,
                             owl:FunctionalProperty ;
                    rdfs:domain :ParameterRange ;
                    rdfs:range :ParameterRange ;
                    rdfs:comment "Relates a comfort envelop with an environmental parameter."@en ;
                    rdfs:label "describes parameter"@en .


###  http://bimerr.iot.linkeddata.es/def/occupancy-profile#detailedBy
:detailedBy rdf:type owl:ObjectProperty ,
                     owl:FunctionalProperty ;
            rdfs:comment "Relates a spatial driver to an specific building space"@en ;
            rdfs:label "detailed by"@en .


###  http://bimerr.iot.linkeddata.es/def/occupancy-profile#drivenBy
:drivenBy rdf:type owl:ObjectProperty ;
          rdfs:domain :Behavior ;
          rdfs:range :DriverSet ;
          rdfs:comment "Property to link an occupant with a set of internal or external drivers that are controlling its interactions with building systems."@en ;
          rdfs:label "driven by"@en .


###  http://bimerr.iot.linkeddata.es/def/occupancy-profile#hasBehavior
:hasBehavior rdf:type owl:ObjectProperty ;
             rdfs:domain :Occupant ;
             rdfs:range :Behavior ;
             rdfs:comment "Property to indicate that an occupant has a behavior."@en ;
             rdfs:label "has behavior"@en .


###  http://bimerr.iot.linkeddata.es/def/occupancy-profile#hasCoefficient
:hasCoefficient rdf:type owl:ObjectProperty ;
                rdfs:domain :InteractionFormula ;
                rdfs:range :Coefficient ;
                rdfs:comment "Relates a formula with a coefficient."@en ;
                rdfs:label "has coefficient"@en .


###  http://bimerr.iot.linkeddata.es/def/occupancy-profile#hasDayOfWeek
:hasDayOfWeek rdf:type owl:ObjectProperty ,
                       owl:FunctionalProperty ;
              rdfs:domain :Time ;
              rdfs:range <http://www.w3.org/2006/time#DayOfWeek> ;
              rdfs:comment "Indicates which days of the week are behavioral drivers for an occupant."@en ;
              rdfs:label "has day of week"@en .


###  http://bimerr.iot.linkeddata.es/def/occupancy-profile#hasEnvironmentalParameter
:hasEnvironmentalParameter rdf:type owl:ObjectProperty ;
                           rdfs:domain :Environment ;
                           rdfs:range :EnvironmentalParameter ;
                           rdfs:comment "Relates and occupant environmental driver with an environmental property like temperature or illuminance."@en ;
                           rdfs:label "has environmental parameter"@en .


###  http://bimerr.iot.linkeddata.es/def/occupancy-profile#hasIndependentVariable
:hasIndependentVariable rdf:type owl:ObjectProperty ;
                        rdfs:domain :InteractionFormula ;
                        rdfs:range :EnvironmentalParameter ;
                        rdfs:comment "Relates a formula with an independent variable."@en ;
                        rdfs:label "has independent variable"@en .


###  http://bimerr.iot.linkeddata.es/def/occupancy-profile#hasMeeting
:hasMeeting rdf:type owl:ObjectProperty ;
            rdfs:domain <http://bimerr.iot.linkeddata.es/def/building#BuildingSpace> ;
            rdfs:range :Meeting ;
            rdfs:comment "Indicates that a meeting can occur within a space."@en ;
            rdfs:label "has meeting"@en .


###  http://bimerr.iot.linkeddata.es/def/occupancy-profile#hasOccupant
:hasOccupant rdf:type owl:ObjectProperty ;
             rdfs:domain <http://bimerr.iot.linkeddata.es/def/building#BuildingSpace> ;
             rdfs:range :Occupant ;
             rdfs:comment "Relationship that indicates that an space can have an occupant."@en ;
             rdfs:label "has occupant"@en .


###  http://bimerr.iot.linkeddata.es/def/occupancy-profile#hasOperationalMode
:hasOperationalMode rdf:type owl:ObjectProperty ;
                    rdfs:domain <https://w3id.org/def/saref4building#PhysicalObject> ;
                    rdfs:range :OperationalModeConcept ;
                    rdfs:comment "Relationship to indicate the type of control mode of a system, such as fixed or operable modes for a window."@en ;
                    rdfs:label "has operational mode"@en .


###  http://bimerr.iot.linkeddata.es/def/occupancy-profile#hasSeason
:hasSeason rdf:type owl:ObjectProperty ,
                    owl:FunctionalProperty ;
           rdfs:domain :Time ;
           rdfs:range :Season ;
           rdfs:comment "Indicates which seasons are behavioral drivers for an occupant."@en ;
           rdfs:label "has season"@en .


###  http://bimerr.iot.linkeddata.es/def/occupancy-profile#hasTimeOfDay
:hasTimeOfDay rdf:type owl:ObjectProperty ,
                       owl:FunctionalProperty ;
              rdfs:domain :Time ;
              rdfs:range :TimeOfDay ;
              rdfs:comment "Indicates which times during a day are behavioral drivers for an occupant."@en ;
              rdfs:label "has time of day"@en .


###  http://bimerr.iot.linkeddata.es/def/occupancy-profile#hasTransitionType
:hasTransitionType rdf:type owl:ObjectProperty ;
                   rdfs:domain :StatusTransition ;
                   rdfs:range :StatusTransitionTypeConcept ;
                   rdfs:comment "Relationship that indicates the type of status transition event."@en ;
                   rdfs:label "has transition type"@en .


###  http://bimerr.iot.linkeddata.es/def/occupancy-profile#hasUnitOfMeasure
:hasUnitOfMeasure rdf:type owl:ObjectProperty ,
                           owl:FunctionalProperty ;
                  rdfs:range <https://w3id.org/saref#UnitOfMeasure> ;
                  rdfs:comment "Relates an environmental parameter with a unit of measure."@en ;
                  rdfs:label "has unit of measure"@en .


###  http://bimerr.iot.linkeddata.es/def/occupancy-profile#influencedByNeed
:influencedByNeed rdf:type owl:ObjectProperty ;
                  rdfs:domain :Behavior ;
                  rdfs:range :Need ;
                  rdfs:comment "Indicates that a driver can be influenced by an occupant comfort need."@en ;
                  rdfs:label "influenced by need"@en .


###  http://bimerr.iot.linkeddata.es/def/occupancy-profile#interactsOver
:interactsOver rdf:type owl:ObjectProperty ,
                        owl:FunctionalProperty ;
               rdfs:domain :Interaction ;
               rdfs:range <https://w3id.org/def/saref4building#PhysicalObject> ;
               rdfs:comment "Relationship that describes an interaction between an occupant and a building component or system."@en ;
               rdfs:label "interacts over"@en .


###  http://bimerr.iot.linkeddata.es/def/occupancy-profile#leadsTo
:leadsTo rdf:type owl:ObjectProperty ;
         rdfs:domain :Behavior ;
         rdfs:comment "Relationship to indicate the outcome of a behavior. It could lead to an action over a building system to recover comfort or to a passive acceptance of the environmental conditions."@en ;
         rdfs:label "leads to"@en .


###  http://bimerr.iot.linkeddata.es/def/occupancy-profile#relatedToSpace
:relatedToSpace rdf:type owl:ObjectProperty ;
                rdfs:range <http://bimerr.iot.linkeddata.es/def/building#BuildingSpace> ;
                rdfs:comment "Property that relates space occupancy events to an specific building space."@en ;
                rdfs:label "related to space"@en .


###  http://bimerr.iot.linkeddata.es/def/occupancy-profile#specifiedBy
:specifiedBy rdf:type owl:ObjectProperty ;
             rdfs:comment "Relates a transition event to a movement model that describe this action."@en ;
             rdfs:label "specified by"@en .


###  http://www.w3.org/2004/02/skos/core#broader
<http://www.w3.org/2004/02/skos/core#broader> rdf:type owl:ObjectProperty ;
                                              rdfs:domain <http://www.w3.org/2004/02/skos/core#Concept> ;
                                              rdfs:range <http://www.w3.org/2004/02/skos/core#Concept> ;
                                              rdfs:label "broader"@en .


###  http://www.w3.org/2004/02/skos/core#inScheme
<http://www.w3.org/2004/02/skos/core#inScheme> rdf:type owl:ObjectProperty ;
                                               rdfs:domain <http://www.w3.org/2004/02/skos/core#Concept> ;
                                               rdfs:range <http://www.w3.org/2004/02/skos/core#ConceptScheme> ;
                                               rdfs:label "in scheme"@en .


###  http://www.w3.org/2004/02/skos/core#narrower
<http://www.w3.org/2004/02/skos/core#narrower> rdf:type owl:ObjectProperty ;
                                               rdfs:domain <http://www.w3.org/2004/02/skos/core#Concept> ;
                                               rdfs:range <http://www.w3.org/2004/02/skos/core#Concept> ;
                                               rdfs:label "narrower"@en .


###  https://w3id.org/def/saref4building#contains
<https://w3id.org/def/saref4building#contains> rdf:type owl:ObjectProperty ;
                                               rdfs:comment "A relation between a physical space and the objects located in such space."@en ;
                                               rdfs:label "contains"@en .


###  https://w3id.org/def/saref4building#hasSpace
<https://w3id.org/def/saref4building#hasSpace> rdf:type owl:ObjectProperty ;
                                               rdfs:comment "Relation between a building or a building space and the spaces it can be divided into."@en ;
                                               rdfs:label "has space"@en .


#################################################################
#    Data properties
#################################################################

###  http://bimerr.iot.linkeddata.es/def/occupancy-profile#buildingAddress
:buildingAddress rdf:type owl:DatatypeProperty ;
                 rdfs:range xsd:string ;
                 rdfs:comment "A relationship indicating the address of a building"@en ;
                 rdfs:label "building address"@en .


###  http://bimerr.iot.linkeddata.es/def/occupancy-profile#coefficientValue
:coefficientValue rdf:type owl:DatatypeProperty ;
                  rdfs:range xsd:float ;
                  rdfs:comment "A relationship indicating the value of a coefficient."@en ;
                  rdfs:label "coefficient value"@en .


###  http://bimerr.iot.linkeddata.es/def/occupancy-profile#controlValue
:controlValue rdf:type owl:DatatypeProperty ;
              rdfs:range xsd:float ;
              rdfs:comment "A relationship indicating the magnitud of a control action over a building system."@en ;
              rdfs:label "control value"@en .


###  http://bimerr.iot.linkeddata.es/def/occupancy-profile#duration
:duration rdf:type owl:DatatypeProperty ;
          rdfs:range xsd:duration ;
          rdfs:comment "Average duration of an event."@en ;
          rdfs:label "duration"@en .


###  http://bimerr.iot.linkeddata.es/def/occupancy-profile#earlyOccurTime
:earlyOccurTime rdf:type owl:DatatypeProperty ;
                rdfs:range xsd:time ;
                rdfs:comment "Earliest occurrence time of an event."@en ;
                rdfs:label "early occur time"@en .


###  http://bimerr.iot.linkeddata.es/def/occupancy-profile#endSeason
:endSeason rdf:type owl:DatatypeProperty ;
           rdfs:domain :Season ;
           rdfs:range xsd:gMonthDay ;
           rdfs:comment "Relationship that indicates the month when a season ends."@en ;
           rdfs:label "end season"@en .


###  http://bimerr.iot.linkeddata.es/def/occupancy-profile#endTime
:endTime rdf:type owl:DatatypeProperty ;
         rdfs:range xsd:dateTime ;
         rdfs:comment "The end time of an event or activity."@en ;
         rdfs:label "end time"@en .


###  http://bimerr.iot.linkeddata.es/def/occupancy-profile#identifier
:identifier rdf:type owl:DatatypeProperty ,
                     owl:FunctionalProperty ;
            rdfs:comment "Identifier of an element given in the obXML file. Attribute considered for backward compatibility."@en ;
            rdfs:label "identifier"@en .


###  http://bimerr.iot.linkeddata.es/def/occupancy-profile#maxNumberOccupants
:maxNumberOccupants rdf:type owl:DatatypeProperty ,
                             owl:FunctionalProperty ;
                    rdfs:range xsd:integer ;
                    rdfs:comment "Relationship that indicates the maximum number of occupants inside a space."@en ;
                    rdfs:label "max number occupants"@en .


###  http://bimerr.iot.linkeddata.es/def/occupancy-profile#maxRangeValue
:maxRangeValue rdf:type owl:DatatypeProperty ,
                        owl:FunctionalProperty ;
               rdfs:range xsd:float ;
               rdfs:comment "Upper boundary of a parameter range description."@en ;
               rdfs:label "max range value"@en .


###  http://bimerr.iot.linkeddata.es/def/occupancy-profile#minNumberOccupants
:minNumberOccupants rdf:type owl:DatatypeProperty ,
                             owl:FunctionalProperty ;
                    rdfs:range xsd:integer ;
                    rdfs:comment "Relationship that indicates the minimum number of occupants inside a space."@en ;
                    rdfs:label "min number occupants"@en .


###  http://bimerr.iot.linkeddata.es/def/occupancy-profile#minRangeValue
:minRangeValue rdf:type owl:DatatypeProperty ,
                        owl:FunctionalProperty ;
               rdfs:range xsd:float ;
               rdfs:comment "Lower boundary of a parameter range description."@en ;
               rdfs:label "min range value"@en .


###  http://bimerr.iot.linkeddata.es/def/occupancy-profile#minimalDuration
:minimalDuration rdf:type owl:DatatypeProperty ;
                 rdfs:range xsd:duration ;
                 rdfs:comment "The minimal duration of an event."@en ;
                 rdfs:label "minimal duration"@en .


###  http://bimerr.iot.linkeddata.es/def/occupancy-profile#occupantAge
:occupantAge rdf:type owl:DatatypeProperty ,
                      owl:FunctionalProperty ;
             rdfs:domain :Occupant ;
             rdfs:range xsd:integer ;
             rdfs:comment "Age of an occupant"@en ;
             rdfs:label "occupant age"@en .


###  http://bimerr.iot.linkeddata.es/def/occupancy-profile#occupantGender
:occupantGender rdf:type owl:DatatypeProperty ,
                         owl:FunctionalProperty ;
                rdfs:domain :Occupant ;
                rdfs:range xsd:string ;
                rdfs:comment "Gender of an occupant"@en ;
                rdfs:label "occupant gender"@en .


###  http://bimerr.iot.linkeddata.es/def/occupancy-profile#occupantJobtype
:occupantJobtype rdf:type owl:DatatypeProperty ,
                          owl:FunctionalProperty ;
                 rdfs:domain :Occupant ;
                 rdfs:range xsd:string ;
                 rdfs:comment "Jobtype of an occupant"@en ;
                 rdfs:label "occupant jobtype"@en .


###  http://bimerr.iot.linkeddata.es/def/occupancy-profile#occupantLifestyle
:occupantLifestyle rdf:type owl:DatatypeProperty ,
                            owl:FunctionalProperty ;
                   rdfs:domain :Occupant ;
                   rdfs:range xsd:string ;
                   rdfs:comment "Lifestyle of an occupant"@en ;
                   rdfs:label "occupant lifestyle"@en .


###  http://bimerr.iot.linkeddata.es/def/occupancy-profile#onHolidays
:onHolidays rdf:type owl:DatatypeProperty ;
            rdfs:range xsd:date ;
            rdfs:comment "Indicates which days that act as time drivers are holidays."@en ;
            rdfs:label "on holidays"@en .


###  http://bimerr.iot.linkeddata.es/def/occupancy-profile#percentTimePresence
:percentTimePresence rdf:type owl:DatatypeProperty ;
                     rdfs:range xsd:float ;
                     rdfs:comment "Percentage of occupancy time in a space."@en ;
                     rdfs:label "percent time presence"@en .


###  http://bimerr.iot.linkeddata.es/def/occupancy-profile#probability
:probability rdf:type owl:DatatypeProperty ;
             rdfs:range xsd:float ;
             rdfs:comment "Relationship that links a probility to an event. For example the occurance probability of a meeting."@en ;
             rdfs:label "probability"@en .


###  http://bimerr.iot.linkeddata.es/def/occupancy-profile#startSeason
:startSeason rdf:type owl:DatatypeProperty ;
             rdfs:domain :Season ;
             rdfs:range xsd:gMonthDay ;
             rdfs:comment "Relationship that indicates the month when a season start."@en ;
             rdfs:label "start season"@en .


###  http://bimerr.iot.linkeddata.es/def/occupancy-profile#startTime
:startTime rdf:type owl:DatatypeProperty ;
           rdfs:range xsd:dateTime ;
           rdfs:comment "The start time of an event or activity."@en ;
           rdfs:label "start time"@en .


###  http://bimerr.iot.linkeddata.es/def/occupancy-profile#typicalDuration
:typicalDuration rdf:type owl:DatatypeProperty ;
                 rdfs:range xsd:duration ;
                 rdfs:comment "The typical duration of an event or activity."@en ;
                 rdfs:label "typical duration"@en .


###  http://bimerr.iot.linkeddata.es/def/occupancy-profile#typicalTime
:typicalTime rdf:type owl:DatatypeProperty ;
             rdfs:range xsd:time ;
             rdfs:comment "Typical occurrence time of an event."@en ;
             rdfs:label "typical time"@en .


#################################################################
#    Classes
#################################################################

###  http://bimerr.iot.linkeddata.es/def/building#Building
<http://bimerr.iot.linkeddata.es/def/building#Building> rdf:type owl:Class ;
                                                        rdfs:subClassOf [ rdf:type owl:Restriction ;
                                                                          owl:onProperty <https://w3id.org/def/saref4building#hasSpace> ;
                                                                          owl:someValuesFrom <http://bimerr.iot.linkeddata.es/def/building#BuildingSpace>
                                                                        ] ,
                                                                        [ rdf:type owl:Restriction ;
                                                                          owl:onProperty :buildingAddress ;
                                                                          owl:someValuesFrom xsd:string
                                                                        ] ,
                                                                        [ rdf:type owl:Restriction ;
                                                                          owl:onProperty :identifier ;
                                                                          owl:someValuesFrom xsd:string
                                                                        ] ;
                                                        rdfs:comment "Building where the occupancy behaviors occur."@en ;
                                                        rdfs:label "Building"@en .


###  http://bimerr.iot.linkeddata.es/def/building#BuildingSpace
<http://bimerr.iot.linkeddata.es/def/building#BuildingSpace> rdf:type owl:Class ;
                                                             rdfs:subClassOf [ rdf:type owl:Restriction ;
                                                                               owl:onProperty <https://w3id.org/def/saref4building#contains> ;
                                                                               owl:someValuesFrom <https://w3id.org/def/saref4building#PhysicalObject>
                                                                             ] ,
                                                                             [ rdf:type owl:Restriction ;
                                                                               owl:onProperty :hasMeeting ;
                                                                               owl:allValuesFrom :Meeting
                                                                             ] ,
                                                                             [ rdf:type owl:Restriction ;
                                                                               owl:onProperty :hasOccupant ;
                                                                               owl:allValuesFrom :Occupant
                                                                             ] ,
                                                                             [ rdf:type owl:Restriction ;
                                                                               owl:onProperty :identifier ;
                                                                               owl:someValuesFrom xsd:string
                                                                             ] ,
                                                                             [ rdf:type owl:Restriction ;
                                                                               owl:onProperty :maxNumberOccupants ;
                                                                               owl:allValuesFrom xsd:integer
                                                                             ] ,
                                                                             [ rdf:type owl:Restriction ;
                                                                               owl:onProperty :minNumberOccupants ;
                                                                               owl:allValuesFrom xsd:integer
                                                                             ] ;
                                                             rdfs:comment "Class to represent the different spaces the building have and where the occupant behaviors occur." ;
                                                             rdfs:label "Space"@en .


###  http://bimerr.iot.linkeddata.es/def/occupancy-profile#AccousticNeed
:AccousticNeed rdf:type owl:Class ;
               rdfs:subClassOf :PhysicalNeed ;
               rdfs:comment "Range of parameter values where occupants do not feel accoustic discomfort and therefore, they don't carry out any actions."@en ;
               rdfs:label "Accoustic Need"@en .


###  http://bimerr.iot.linkeddata.es/def/occupancy-profile#Action
:Action rdf:type owl:Class ;
        rdfs:comment "Actions are the interactions with systems or activities that an occupant can conduct to achieve environmental comfort. Actions connect occupants' inside-world needs with the environmental outside world. (Defintion taken from obXML)"@en ;
        rdfs:label "Action"@en .


###  http://bimerr.iot.linkeddata.es/def/occupancy-profile#Behavior
:Behavior rdf:type owl:Class ;
          rdfs:subClassOf [ rdf:type owl:Restriction ;
                            owl:onProperty :drivenBy ;
                            owl:someValuesFrom :DriverSet
                          ] ,
                          [ rdf:type owl:Restriction ;
                            owl:onProperty :leadsTo ;
                            owl:someValuesFrom [ rdf:type owl:Class ;
                                                 owl:unionOf ( :Action
                                                               :Inaction
                                                             )
                                               ]
                          ] ,
                          [ rdf:type owl:Restriction ;
                            owl:onProperty :influencedByNeed ;
                            owl:allValuesFrom :Need
                          ] ,
                          [ rdf:type owl:Restriction ;
                            owl:onProperty :identifier ;
                            owl:someValuesFrom xsd:string
                          ] ;
          rdfs:comment "Behavior related to the interaction with buildings"@en ;
          rdfs:label "Behavior"@en .


###  http://bimerr.iot.linkeddata.es/def/occupancy-profile#Coefficient
:Coefficient rdf:type owl:Class ;
             rdfs:subClassOf [ rdf:type owl:Restriction ;
                               owl:onProperty :coefficientValue ;
                               owl:someValuesFrom xsd:float
                             ] ;
             rdfs:comment "Class to represent the value and name of coefficients inside mathematical formulas."@en ;
             rdfs:label "Coefficient"@en .


###  http://bimerr.iot.linkeddata.es/def/occupancy-profile#ConstantValueFormula
:ConstantValueFormula rdf:type owl:Class ;
                      rdfs:subClassOf :InteractionFormula ;
                      rdfs:comment "Class to represent constant value mathematical formulas"@en ;
                      rdfs:label "Constant Value Formula"@en .


###  http://bimerr.iot.linkeddata.es/def/occupancy-profile#CustomProbabilityModel
:CustomProbabilityModel rdf:type owl:Class ;
                        rdfs:subClassOf :MovementModel ,
                                        [ rdf:type owl:Restriction ;
                                          owl:onProperty :probability ;
                                          owl:someValuesFrom xsd:float
                                        ] ;
                        rdfs:comment "Class to represent instances of custom probabilistic models."@en ;
                        rdfs:label "Custom probability model"@en .


###  http://bimerr.iot.linkeddata.es/def/occupancy-profile#Driver
:Driver rdf:type owl:Class ;
        rdfs:comment "A Driver represents the environmental factor from the outside world that stimulate occupants in their inside world to fulfill a physical, physiological or psychological need."@en ;
        rdfs:label "Driver"@en .


###  http://bimerr.iot.linkeddata.es/def/occupancy-profile#DriverSet
:DriverSet rdf:type owl:Class ;
           rdfs:subClassOf [ rdf:type owl:Restriction ;
                             owl:onProperty :composedOf ;
                             owl:someValuesFrom :Driver
                           ] ;
           rdfs:comment "Set of drivers that could be causing a behavior at a specific time."@en ;
           rdfs:label "Driver set"@en .


###  http://bimerr.iot.linkeddata.es/def/occupancy-profile#Environment
:Environment rdf:type owl:Class ;
             rdfs:subClassOf :Driver ,
                             [ rdf:type owl:Restriction ;
                               owl:onProperty :hasEnvironmentalParameter ;
                               owl:someValuesFrom :EnvironmentalParameter
                             ] ;
             rdfs:comment "Driver related to the environmental conditions that could be causing a behavior."@en ;
             rdfs:label "Environment"@en .


###  http://bimerr.iot.linkeddata.es/def/occupancy-profile#EnvironmentalParameter
:EnvironmentalParameter rdf:type owl:Class ;
                        rdfs:subClassOf <https://w3id.org/saref#Property> ,
                                        [ rdf:type owl:Restriction ;
                                          owl:onProperty :hasUnitOfMeasure ;
                                          owl:someValuesFrom <https://w3id.org/saref#UnitOfMeasure>
                                        ] ,
                                        [ rdf:type owl:Restriction ;
                                          owl:onProperty :identifier ;
                                          owl:someValuesFrom xsd:string
                                        ] ;
                        rdfs:comment "Class that represent a physical variable of the environment where the driver occurs. It could represent variables that impact directly on the comfort levels of the occupant."@en ;
                        rdfs:label "Environmental parameter"@en .


###  http://bimerr.iot.linkeddata.es/def/occupancy-profile#Equipment
:Equipment rdf:type owl:Class ;
           rdfs:subClassOf <https://w3id.org/saref#Device> ;
           rdfs:comment "Class to represent electrical equipments occupants interact with but do not have influence over indoor thermal conditions. These systems contribute to the energy bugdet estimation."@en ;
           rdfs:label "Equipment"@en .


###  http://bimerr.iot.linkeddata.es/def/occupancy-profile#Event
:Event rdf:type owl:Class ;
       rdfs:subClassOf :Driver ;
       rdfs:comment "Driver related to events that could be causing a behavior."@en ;
       rdfs:label "Event"@en .


###  http://bimerr.iot.linkeddata.es/def/occupancy-profile#Habit
:Habit rdf:type owl:Class ;
       rdfs:subClassOf :Driver ;
       rdfs:comment "Driver related to habits that could be causing a behavior."@en ;
       rdfs:label "Habit"@en .


###  http://bimerr.iot.linkeddata.es/def/occupancy-profile#IAQNeed
:IAQNeed rdf:type owl:Class ;
         rdfs:subClassOf :PhysicalNeed ;
         rdfs:comment "Range of parameter values where occupants do not feel indoor air quality discomfort and therefore, they don't carry out any actions."@en ;
         rdfs:label "IAQ Need"@en .


###  http://bimerr.iot.linkeddata.es/def/occupancy-profile#Inaction
:Inaction rdf:type owl:Class .


###  http://bimerr.iot.linkeddata.es/def/occupancy-profile#Interaction
:Interaction rdf:type owl:Class ;
             rdfs:subClassOf :Action ,
                             [ rdf:type owl:Restriction ;
                               owl:onProperty :describedByFormula ;
                               owl:someValuesFrom :InteractionFormula
                             ] ,
                             [ rdf:type owl:Restriction ;
                               owl:onProperty :interactsOver ;
                               owl:someValuesFrom <https://w3id.org/def/saref4building#BuildingObject>
                             ] ,
                             [ rdf:type owl:Restriction ;
                               owl:onProperty :controlValue ;
                               owl:someValuesFrom xsd:float
                             ] ;
             rdfs:comment "The Interaction class represent the interactions of occupants with systems within a space to recover their comfort."@en ;
             rdfs:label "Interaction"@en .


###  http://bimerr.iot.linkeddata.es/def/occupancy-profile#InteractionConcept
:InteractionConcept rdf:type owl:Class ;
                    rdfs:subClassOf <http://www.w3.org/2004/02/skos/core#Concept> ;
                    rdfs:comment "Types of interactions between occupants and systems."@en ;
                    rdfs:label "Interaction concept"@en .


###  http://bimerr.iot.linkeddata.es/def/occupancy-profile#InteractionFormula
:InteractionFormula rdf:type owl:Class ;
                    rdfs:subClassOf [ rdf:type owl:Restriction ;
                                      owl:onProperty :hasCoefficient ;
                                      owl:someValuesFrom :Coefficient
                                    ] ,
                                    [ rdf:type owl:Restriction ;
                                      owl:onProperty :hasIndependentVariable ;
                                      owl:someValuesFrom :EnvironmentalParameter
                                    ] ;
                    rdfs:comment "Formula to model the probability of interaction between ocupant and system."@en ;
                    rdfs:label "Interaction Formula"@en .


###  http://bimerr.iot.linkeddata.es/def/occupancy-profile#InteractionScheme
:InteractionScheme rdf:type owl:Class ;
                   rdfs:subClassOf <http://www.w3.org/2004/02/skos/core#ConceptScheme> ;
                   rdfs:comment "An aggregation of SKOS concepts regarding the interaction type between occupants and space systems"@en ;
                   rdfs:label "Interaction scheme"@en .


###  http://bimerr.iot.linkeddata.es/def/occupancy-profile#LightingDevice
:LightingDevice rdf:type owl:Class ;
                rdfs:subClassOf <https://w3id.org/saref#Device> ;
                rdfs:comment "A devide used for illumination."@en ;
                rdfs:label "Lighting device"@en .


###  http://bimerr.iot.linkeddata.es/def/occupancy-profile#LinearFormula
:LinearFormula rdf:type owl:Class ;
               rdfs:subClassOf :InteractionFormula ;
               rdfs:comment "Class to represent linear mathematical formulas"@en ;
               rdfs:label "Linear Formula"@en .


###  http://bimerr.iot.linkeddata.es/def/occupancy-profile#LogitFormula
:LogitFormula rdf:type owl:Class ;
              rdfs:subClassOf :InteractionFormula ;
              rdfs:comment "Class to represent logit mathematical formulas."@en ;
              rdfs:label "Logit Formula"@en .


###  http://bimerr.iot.linkeddata.es/def/occupancy-profile#MarkovChainModel
:MarkovChainModel rdf:type owl:Class ;
                  rdfs:subClassOf :MovementModel ,
                                  [ rdf:type owl:Restriction ;
                                    owl:onProperty :earlyOccurTime ;
                                    owl:someValuesFrom xsd:time
                                  ] ,
                                  [ rdf:type owl:Restriction ;
                                    owl:onProperty :typicalTime ;
                                    owl:someValuesFrom xsd:time
                                  ] ;
                  rdfs:comment "Class to represent instances of Markov chain models."@en ;
                  rdfs:label "Markov chain model"@en .


###  http://bimerr.iot.linkeddata.es/def/occupancy-profile#Meeting
:Meeting rdf:type owl:Class ;
         rdfs:subClassOf [ rdf:type owl:Restriction ;
                           owl:onProperty :duration ;
                           owl:someValuesFrom xsd:duration
                         ] ,
                         [ rdf:type owl:Restriction ;
                           owl:onProperty :endTime ;
                           owl:someValuesFrom xsd:dateTime
                         ] ,
                         [ rdf:type owl:Restriction ;
                           owl:onProperty :probability ;
                           owl:someValuesFrom xsd:float
                         ] ,
                         [ rdf:type owl:Restriction ;
                           owl:onProperty :startTime ;
                           owl:someValuesFrom xsd:dateTime
                         ] ;
         rdfs:comment "Class to represent a meeting inside a communal space."@en ;
         rdfs:label "Meeting"@en .


###  http://bimerr.iot.linkeddata.es/def/occupancy-profile#Movement
:Movement rdf:type owl:Class ;
          rdfs:subClassOf <http://xmlns.com/foaf/0.1#Person> ;
          rdfs:comment "The Movement class is used to represent the occupant's movements inside or between spaces."@en ;
          rdfs:label "Movement"@en .


###  http://bimerr.iot.linkeddata.es/def/occupancy-profile#MovementModel
:MovementModel rdf:type owl:Class ;
               rdfs:comment "Probabilistic model to define occupant movements inside and between spaces."@en ;
               rdfs:label "Movement Model"@en .


###  http://bimerr.iot.linkeddata.es/def/occupancy-profile#Need
:Need rdf:type owl:Class ;
      rdfs:comment "Needs represent the physical and non-physical requirements of the occupant's inside world that must be met in order to ensure the satisfaction of the occupant with their environment."@en ;
      rdfs:label "Need"@en .


###  http://bimerr.iot.linkeddata.es/def/occupancy-profile#NonPhysicalNeed
:NonPhysicalNeed rdf:type owl:Class ;
                 rdfs:subClassOf :Need ;
                 owl:disjointWith :PhysicalNeed ;
                 rdfs:comment "Non physical comfort needs (e.g. privacy, status, etc) that could influence a behavior."@en ;
                 rdfs:label "Non Physical Need"@en .


###  http://bimerr.iot.linkeddata.es/def/occupancy-profile#NormalProbabilityModel
:NormalProbabilityModel rdf:type owl:Class ;
                        rdfs:subClassOf :MovementModel ,
                                        [ rdf:type owl:Restriction ;
                                          owl:onProperty :earlyOccurTime ;
                                          owl:someValuesFrom xsd:time
                                        ] ,
                                        [ rdf:type owl:Restriction ;
                                          owl:onProperty :typicalTime ;
                                          owl:someValuesFrom xsd:time
                                        ] ;
                        rdfs:comment "Class to represent instances of Normal probabilistic models."@en ;
                        rdfs:label "Normal probability model"@en .


###  http://bimerr.iot.linkeddata.es/def/occupancy-profile#Occupant
:Occupant rdf:type owl:Class ;
          rdfs:subClassOf <http://xmlns.com/foaf/0.1#Person> ,
                          [ rdf:type owl:Restriction ;
                            owl:onProperty :hasBehavior ;
                            owl:someValuesFrom :Behavior
                          ] ,
                          [ rdf:type owl:Restriction ;
                            owl:onProperty :identifier ;
                            owl:someValuesFrom xsd:string
                          ] ,
                          [ rdf:type owl:Restriction ;
                            owl:onProperty :occupantAge ;
                            owl:allValuesFrom xsd:integer
                          ] ,
                          [ rdf:type owl:Restriction ;
                            owl:onProperty :occupantGender ;
                            owl:allValuesFrom xsd:string
                          ] ,
                          [ rdf:type owl:Restriction ;
                            owl:onProperty :occupantJobtype ;
                            owl:allValuesFrom xsd:string
                          ] ,
                          [ rdf:type owl:Restriction ;
                            owl:onProperty :occupantLifestyle ;
                            owl:allValuesFrom xsd:string
                          ] ;
          rdfs:comment "Occupants or residents of a building."@en ;
          rdfs:label "Occupant"@en .


###  http://bimerr.iot.linkeddata.es/def/occupancy-profile#OperationalModeConcept
:OperationalModeConcept rdf:type owl:Class ;
                        rdfs:subClassOf <http://www.w3.org/2004/02/skos/core#Concept> ;
                        rdfs:comment "Types of operational modes for space systems."@en ;
                        rdfs:label "Operational mode concept"@en .


###  http://bimerr.iot.linkeddata.es/def/occupancy-profile#OperationalModeConceptScheme
:OperationalModeConceptScheme rdf:type owl:Class ;
                              rdfs:subClassOf <http://www.w3.org/2004/02/skos/core#ConceptScheme> ;
                              rdfs:comment "An aggregation of SKOS concepts regarding the operational mode of space systems."@en ;
                              rdfs:label "Operational mode scheme"@en .


###  http://bimerr.iot.linkeddata.es/def/occupancy-profile#ParameterRange
:ParameterRange rdf:type owl:Class ;
                rdfs:subClassOf [ rdf:type owl:Restriction ;
                                  owl:onProperty :describesParameter ;
                                  owl:someValuesFrom :EnvironmentalParameter
                                ] ,
                                [ rdf:type owl:Restriction ;
                                  owl:onProperty :maxRangeValue ;
                                  owl:someValuesFrom xsd:float
                                ] ,
                                [ rdf:type owl:Restriction ;
                                  owl:onProperty :minRangeValue ;
                                  owl:someValuesFrom xsd:float
                                ] ;
                rdfs:comment "Class to represent the minimum and maximm comfort values with respect to an environmental parameter."@en ;
                rdfs:label "Parameter Range"@en .


###  http://bimerr.iot.linkeddata.es/def/occupancy-profile#PhysicalNeed
:PhysicalNeed rdf:type owl:Class ;
              rdfs:subClassOf :Need ,
                              [ rdf:type owl:Restriction ;
                                owl:onProperty :definedByRange ;
                                owl:someValuesFrom :ParameterRange
                              ] ;
              rdfs:comment "Physical comfort need that could influence a behavior."@en ;
              rdfs:label "Physical Need"@en .


###  http://bimerr.iot.linkeddata.es/def/occupancy-profile#QuadraticFormula
:QuadraticFormula rdf:type owl:Class ;
                  rdfs:subClassOf :InteractionFormula ;
                  rdfs:comment "Class to represent quadratic mathematical formulas."@en ;
                  rdfs:label "Quadratic Formula"@en .


###  http://bimerr.iot.linkeddata.es/def/occupancy-profile#RandomMovement
:RandomMovement rdf:type owl:Class ;
                rdfs:subClassOf :Movement ;
                rdfs:comment "Type of occupant movements inside a building or space."@en ;
                rdfs:label "Random movement"@en .


###  http://bimerr.iot.linkeddata.es/def/occupancy-profile#Report
:Report rdf:type owl:Class ;
        rdfs:subClassOf :Action ;
        rdfs:comment "The Report class indicates that an occupant seeks assistance or files a complaint about their personal discomfort, but does not take direct action to satisfy their needs."@en ;
        rdfs:label "Report"@en .


###  http://bimerr.iot.linkeddata.es/def/occupancy-profile#Season
:Season rdf:type owl:Class ;
        rdfs:subClassOf [ rdf:type owl:Restriction ;
                          owl:onProperty :endSeason ;
                          owl:someValuesFrom xsd:gMonthDay
                        ] ,
                        [ rdf:type owl:Restriction ;
                          owl:onProperty :startSeason ;
                          owl:someValuesFrom xsd:gMonthDay
                        ] ;
        rdfs:comment "Season of the year."@en ;
        rdfs:label "Season"@en .


###  http://bimerr.iot.linkeddata.es/def/occupancy-profile#SpaceOccupancy
:SpaceOccupancy rdf:type owl:Class ;
                rdfs:subClassOf :RandomMovement ,
                                [ rdf:type owl:Restriction ;
                                  owl:onProperty :relatedToSpace ;
                                  owl:someValuesFrom <http://bimerr.iot.linkeddata.es/def/building#BuildingSpace>
                                ] ,
                                [ rdf:type owl:Restriction ;
                                  owl:onProperty :duration ;
                                  owl:someValuesFrom xsd:duration
                                ] ,
                                [ rdf:type owl:Restriction ;
                                  owl:onProperty :percentTimePresence ;
                                  owl:someValuesFrom xsd:float
                                ] ;
                rdfs:comment "Occupancy percentage of staying in a specific space category in a building."@en ;
                rdfs:label "Space occupancy"@en .


###  http://bimerr.iot.linkeddata.es/def/occupancy-profile#Spatial
:Spatial rdf:type owl:Class ;
         rdfs:subClassOf :Driver ,
                         [ rdf:type owl:Restriction ;
                           owl:onProperty :detailedBy ;
                           owl:someValuesFrom <http://bimerr.iot.linkeddata.es/def/building#BuildingSpace>
                         ] ;
         rdfs:comment "Driver related to spatial conditions that could be causing a behavior."@en ;
         rdfs:label "Spatial"@en .


###  http://bimerr.iot.linkeddata.es/def/occupancy-profile#StatusTransition
:StatusTransition rdf:type owl:Class ;
                  rdfs:subClassOf :Movement ,
                                  [ rdf:type owl:Restriction ;
                                    owl:onProperty :hasTransitionType ;
                                    owl:someValuesFrom :StatusTransitionTypeConcept
                                  ] ,
                                  [ rdf:type owl:Restriction ;
                                    owl:onProperty :specifiedBy ;
                                    owl:someValuesFrom :MovementModel
                                  ] ,
                                  [ rdf:type owl:Restriction ;
                                    owl:onProperty :minimalDuration ;
                                    owl:someValuesFrom xsd:duration
                                  ] ,
                                  [ rdf:type owl:Restriction ;
                                    owl:onProperty :typicalDuration ;
                                    owl:someValuesFrom xsd:duration
                                  ] ;
                  rdfs:comment "Type of movements to represent transition events between spaces."@en ;
                  rdfs:label "Status transition"@en .


###  http://bimerr.iot.linkeddata.es/def/occupancy-profile#StatusTransitionScheme
:StatusTransitionScheme rdf:type owl:Class ;
                        rdfs:subClassOf <http://www.w3.org/2004/02/skos/core#ConceptScheme> ;
                        rdfs:comment "An aggregation of SKOS concepts regarding the status transition type of movements between spaces."@en ;
                        rdfs:label "Status transition scheme"@en .


###  http://bimerr.iot.linkeddata.es/def/occupancy-profile#StatusTransitionTypeConcept
:StatusTransitionTypeConcept rdf:type owl:Class ;
                             rdfs:subClassOf <http://www.w3.org/2004/02/skos/core#Concept> ;
                             rdfs:comment "One time event involving occupancy status transition in building level."@en ;
                             rdfs:label "Status transition type concept"@en .


###  http://bimerr.iot.linkeddata.es/def/occupancy-profile#ThermalNeed
:ThermalNeed rdf:type owl:Class ;
             rdfs:subClassOf :PhysicalNeed ;
             rdfs:comment "Range of parameter values where occupants do not feel thermal discomfort and therefore, they don't carry out any actions."@en ;
             rdfs:label "Thermal Need"@en .


###  http://bimerr.iot.linkeddata.es/def/occupancy-profile#Thermostat
:Thermostat rdf:type owl:Class ;
            rdfs:subClassOf <https://w3id.org/def/saref4building#UnitaryControlElement> ;
            rdfs:comment "A thermostat is a component which senses the temperature of a physical space and performs actions so that the space temperature is maintained near a desired setpoint. (Definition adapted from Wikipedia)"@en ;
            rdfs:label "Thermostat"@en .


###  http://bimerr.iot.linkeddata.es/def/occupancy-profile#Time
:Time rdf:type owl:Class ;
      rdfs:subClassOf :Driver ,
                      [ rdf:type owl:Restriction ;
                        owl:onProperty :hasDayOfWeek ;
                        owl:allValuesFrom <http://www.w3.org/2006/time#DayOfWeek>
                      ] ,
                      [ rdf:type owl:Restriction ;
                        owl:onProperty :hasSeason ;
                        owl:allValuesFrom :Season
                      ] ,
                      [ rdf:type owl:Restriction ;
                        owl:onProperty :hasTimeOfDay ;
                        owl:allValuesFrom :TimeOfDay
                      ] ,
                      [ rdf:type owl:Restriction ;
                        owl:onProperty :onHolidays ;
                        owl:allValuesFrom xsd:date
                      ] ;
      rdfs:comment "Driver related to time conditions that could be causing a behavior. It also describes the time when another type of driver occur."@en ;
      rdfs:label "Time"@en .


###  http://bimerr.iot.linkeddata.es/def/occupancy-profile#TimeOfDay
:TimeOfDay rdf:type owl:Class ;
           rdfs:subClassOf [ rdf:type owl:Restriction ;
                             owl:onProperty :endTime ;
                             owl:someValuesFrom xsd:time
                           ] ,
                           [ rdf:type owl:Restriction ;
                             owl:onProperty :startTime ;
                             owl:someValuesFrom xsd:time
                           ] ;
           rdfs:comment "Relative time of day."@en ;
           rdfs:label "Time Of Day"@en .


###  http://bimerr.iot.linkeddata.es/def/occupancy-profile#VisualNeed
:VisualNeed rdf:type owl:Class ;
            rdfs:subClassOf :PhysicalNeed ;
            rdfs:comment "Range of parameter values where occupants do not feel visual discomfort and therefore, they don't carry out any actions."@en ;
            rdfs:label "Visual Need"@en .


###  http://bimerr.iot.linkeddata.es/def/occupancy-profile#WeibullFormula
:WeibullFormula rdf:type owl:Class ;
                rdfs:subClassOf :InteractionFormula ;
                rdfs:comment "Class to represent weibull mathematical formulas."@en ;
                rdfs:label "Weibull Formula"@en .


###  http://bimerr.iot.linkeddata.es/def/occupancy-profile#Window
:Window rdf:type owl:Class ;
        rdfs:subClassOf <https://w3id.org/def/saref4building#BuildingObject> ;
        rdfs:comment "A window is an opening in a wall, door, roof or vehicle that allows the passage of light, sound, and sometimes air. (Definition taken from Wikipedia)"@en ;
        rdfs:label "Window"@en .


###  http://www.w3.org/2004/02/skos/core#Concept
<http://www.w3.org/2004/02/skos/core#Concept> rdf:type owl:Class ;
                                              rdfs:subClassOf [ rdf:type owl:Restriction ;
                                                                owl:onProperty <http://www.w3.org/2004/02/skos/core#broader> ;
                                                                owl:someValuesFrom <http://www.w3.org/2004/02/skos/core#Concept>
                                                              ] ,
                                                              [ rdf:type owl:Restriction ;
                                                                owl:onProperty <http://www.w3.org/2004/02/skos/core#inScheme> ;
                                                                owl:someValuesFrom <http://www.w3.org/2004/02/skos/core#ConceptScheme>
                                                              ] ,
                                                              [ rdf:type owl:Restriction ;
                                                                owl:onProperty <http://www.w3.org/2004/02/skos/core#narrower> ;
                                                                owl:someValuesFrom <http://www.w3.org/2004/02/skos/core#Concept>
                                                              ] ;
                                              rdfs:isDefinedBy <http://www.w3.org/2004/02/skos/core#> ;
                                              rdfs:label "Concept"@en .


###  http://www.w3.org/2004/02/skos/core#ConceptScheme
<http://www.w3.org/2004/02/skos/core#ConceptScheme> rdf:type owl:Class ;
                                                    rdfs:isDefinedBy <http://www.w3.org/2004/02/skos/core#> ;
                                                    rdfs:label "Concept Scheme"@en .


###  http://www.w3.org/2006/time#DayOfWeek
<http://www.w3.org/2006/time#DayOfWeek> rdf:type owl:Class ;
                                        rdfs:comment "The day of the week."@en ;
                                        rdfs:label "Day of week"@en .


###  http://xmlns.com/foaf/0.1#Person
<http://xmlns.com/foaf/0.1#Person> rdf:type owl:Class ;
                                   rdfs:comment "The Person class represents people. Something is a Person if it is a person. We don't nitpic about whether they're alive, dead, real, or imaginary. (Definition taken from FOAF)"@en ;
                                   rdfs:label "Person"@en .


###  https://w3id.org/def/saref4building#BuildingObject
<https://w3id.org/def/saref4building#BuildingObject> rdf:type owl:Class ;
                                                     rdfs:subClassOf <https://w3id.org/def/saref4building#PhysicalObject> ;
                                                     rdfs:comment "An object in the building that can be controlled by devices, such as a door or a window that can be automatically opened or closed by an actuator. (Definition taken from SAREF 1.0)"@en ;
                                                     rdfs:label "Building object"@en .


###  https://w3id.org/def/saref4building#PhysicalObject
<https://w3id.org/def/saref4building#PhysicalObject> rdf:type owl:Class ;
                                                     rdfs:subClassOf [ rdf:type owl:Restriction ;
                                                                       owl:onProperty :hasOperationalMode ;
                                                                       owl:someValuesFrom :OperationalModeConcept
                                                                     ] ;
                                                     rdfs:comment "Any Object that has a proper space region. (Definition extracted from DUL ontology)"@en ;
                                                     rdfs:label "Physical object"@en .


###  https://w3id.org/def/saref4building#ShadingDevice
<https://w3id.org/def/saref4building#ShadingDevice> rdf:type owl:Class ;
                                                    rdfs:subClassOf <https://w3id.org/saref#Device> ;
                                                    rdfs:comment "Shading devices are purpose built devices to protect from the sunlight, from natural light, or screening them from view. Shading devices can form part of the facade or can be mounted inside the building, they can be fixed or operable. (Definition taken from S4BLDG ontology)"@en ;
                                                    rdfs:label "Shading device"@en .


###  https://w3id.org/def/saref4building#UnitaryControlElement
<https://w3id.org/def/saref4building#UnitaryControlElement> rdf:type owl:Class ;
                                                            rdfs:subClassOf <https://w3id.org/saref#Device> ;
                                                            rdfs:comment "A unitary control element provides a housing for an aggregation of control or electrical distribution elements that, in combination, perform a singular (unitary) purpose. Each item in the aggregation may have its own geometric representation and location. (Definition taken from S4BLDG ontology)"@en ;
                                                            rdfs:label "Unitary control element"@en .


###  https://w3id.org/saref#Device
<https://w3id.org/saref#Device> rdf:type owl:Class ;
                                rdfs:subClassOf <https://w3id.org/def/saref4building#PhysicalObject> ;
                                rdfs:comment "A tangible object designed to accomplish a particular task in households, common public buildings or offices. In order to accomplish this task, the device performs one or more functions. For example, a washing machine is designed to wash (task) and to accomplish this task it performs the start and stop function."@en ;
                                rdfs:label "Device"@en .


###  https://w3id.org/saref#HVAC
<https://w3id.org/saref#HVAC> rdf:type owl:Class ;
                              rdfs:subClassOf <https://w3id.org/saref#Device> ;
                              rdfs:comment "Heating, Ventilation and Air Conditioning (HVAC) device that provides indoor environmental comfort. A saref:HVAC is typically used to accomplish saref:Comfort."@en ;
                              rdfs:label "HVAC"@en .


###  https://w3id.org/saref#Property
<https://w3id.org/saref#Property> rdf:type owl:Class ;
                                  rdfs:comment "An aspect of an entity that can be observable by a sensor."@en ;
                                  rdfs:label "Property"@en .


###  https://w3id.org/saref#UnitOfMeasure
<https://w3id.org/saref#UnitOfMeasure> rdf:type owl:Class ;
                                       rdfs:comment "The unit of measure is a standard for measurement of a quantity, such as a Property. For example, Power is a property and Watt is a unit of power that represents a definite predetermined power: when we say 10 Watt, we actually mean 10 times the definite predetermined power called \"watt\". Our definition is based on the definition of unit of measure in the Ontology of units of Measure (OM). We propose here a list of some units of measure that are relevant for the purpose of the Smart Appliances ontology, but this list can be extended."@en ;
                                       rdfs:label "Unit of measure"@en .


#################################################################
#    Individuals
#################################################################

###  http://bimerr.iot.linkeddata.es/def/occupancy-profile#ASHRAEAdaptiveComfort
:ASHRAEAdaptiveComfort rdf:type owl:NamedIndividual ,
                                :ThermalNeed .


###  http://bimerr.iot.linkeddata.es/def/occupancy-profile#ASHRAEComfortEnvelop
:ASHRAEComfortEnvelop rdf:type owl:NamedIndividual ,
                               :ThermalNeed .


###  http://bimerr.iot.linkeddata.es/def/occupancy-profile#Adjustable
:Adjustable rdf:type owl:NamedIndividual ,
                     :OperationalModeConcept .


###  http://bimerr.iot.linkeddata.es/def/occupancy-profile#Afternoon
:Afternoon rdf:type owl:NamedIndividual ,
                    :TimeOfDay .


###  http://bimerr.iot.linkeddata.es/def/occupancy-profile#Arrival
:Arrival rdf:type owl:NamedIndividual ,
                  :StatusTransitionTypeConcept .


###  http://bimerr.iot.linkeddata.es/def/occupancy-profile#ContinuousControl
:ContinuousControl rdf:type owl:NamedIndividual ,
                            :OperationalModeConcept .


###  http://bimerr.iot.linkeddata.es/def/occupancy-profile#Day
:Day rdf:type owl:NamedIndividual ,
              :TimeOfDay .


###  http://bimerr.iot.linkeddata.es/def/occupancy-profile#DayLight
:DayLight rdf:type owl:NamedIndividual ,
                   <https://w3id.org/saref#Property> .


###  http://bimerr.iot.linkeddata.es/def/occupancy-profile#Departure
:Departure rdf:type owl:NamedIndividual ,
                    :StatusTransitionTypeConcept .


###  http://bimerr.iot.linkeddata.es/def/occupancy-profile#EnteringRoom
:EnteringRoom rdf:type owl:NamedIndividual ,
                       :Event .


###  http://bimerr.iot.linkeddata.es/def/occupancy-profile#Evening
:Evening rdf:type owl:NamedIndividual ,
                  :TimeOfDay .


###  http://bimerr.iot.linkeddata.es/def/occupancy-profile#Fall
:Fall rdf:type owl:NamedIndividual ,
               :Season .


###  http://bimerr.iot.linkeddata.es/def/occupancy-profile#Fixed
:Fixed rdf:type owl:NamedIndividual ,
                :OperationalModeConcept .


###  http://bimerr.iot.linkeddata.es/def/occupancy-profile#Glare
:Glare rdf:type owl:NamedIndividual ,
                <https://w3id.org/saref#Property> .


###  http://bimerr.iot.linkeddata.es/def/occupancy-profile#ISOAdaptiveComfort
:ISOAdaptiveComfort rdf:type owl:NamedIndividual ,
                             :ThermalNeed .


###  http://bimerr.iot.linkeddata.es/def/occupancy-profile#Illuminance
:Illuminance rdf:type owl:NamedIndividual ,
                      <https://w3id.org/saref#Property> .


###  http://bimerr.iot.linkeddata.es/def/occupancy-profile#Inaction
:Inaction rdf:type owl:NamedIndividual ,
                   :Inaction .


###  http://bimerr.iot.linkeddata.es/def/occupancy-profile#IndoorAirQuality
:IndoorAirQuality rdf:type owl:NamedIndividual ,
                           <https://w3id.org/saref#Property> .


###  http://bimerr.iot.linkeddata.es/def/occupancy-profile#LeavingRoom
:LeavingRoom rdf:type owl:NamedIndividual ,
                      :Event .


###  http://bimerr.iot.linkeddata.es/def/occupancy-profile#Morning
:Morning rdf:type owl:NamedIndividual ,
                  :TimeOfDay .


###  http://bimerr.iot.linkeddata.es/def/occupancy-profile#Night
:Night rdf:type owl:NamedIndividual ,
                :TimeOfDay .


###  http://bimerr.iot.linkeddata.es/def/occupancy-profile#Noise
:Noise rdf:type owl:NamedIndividual ,
                <https://w3id.org/saref#Property> .


###  http://bimerr.iot.linkeddata.es/def/occupancy-profile#Noon
:Noon rdf:type owl:NamedIndividual ,
               :TimeOfDay .


###  http://bimerr.iot.linkeddata.es/def/occupancy-profile#OnOff
:OnOff rdf:type owl:NamedIndividual ,
                :OperationalModeConcept .


###  http://bimerr.iot.linkeddata.es/def/occupancy-profile#Operable
:Operable rdf:type owl:NamedIndividual ,
                   :OperationalModeConcept .


###  http://bimerr.iot.linkeddata.es/def/occupancy-profile#Rain
:Rain rdf:type owl:NamedIndividual ,
               <https://w3id.org/saref#Property> .


###  http://bimerr.iot.linkeddata.es/def/occupancy-profile#RelativeHumidity
:RelativeHumidity rdf:type owl:NamedIndividual ,
                           <https://w3id.org/saref#Property> .


###  http://bimerr.iot.linkeddata.es/def/occupancy-profile#SetToControlValue
:SetToControlValue rdf:type owl:NamedIndividual ,
                            :InteractionConcept .


###  http://bimerr.iot.linkeddata.es/def/occupancy-profile#ShortTermLeaving
:ShortTermLeaving rdf:type owl:NamedIndividual ,
                           :StatusTransitionTypeConcept .


###  http://bimerr.iot.linkeddata.es/def/occupancy-profile#ShortTermVisiting
:ShortTermVisiting rdf:type owl:NamedIndividual ,
                            :StatusTransitionTypeConcept .


###  http://bimerr.iot.linkeddata.es/def/occupancy-profile#SolarIrradiance
:SolarIrradiance rdf:type owl:NamedIndividual ,
                          <https://w3id.org/saref#Property> .


###  http://bimerr.iot.linkeddata.es/def/occupancy-profile#Spring
:Spring rdf:type owl:NamedIndividual ,
                 :Season .


###  http://bimerr.iot.linkeddata.es/def/occupancy-profile#StayingInRoom
:StayingInRoom rdf:type owl:NamedIndividual ,
                        :Event .


###  http://bimerr.iot.linkeddata.es/def/occupancy-profile#Summer
:Summer rdf:type owl:NamedIndividual ,
                 :Season .


###  http://bimerr.iot.linkeddata.es/def/occupancy-profile#Temperature
:Temperature rdf:type owl:NamedIndividual ,
                      <https://w3id.org/saref#Property> .


###  http://bimerr.iot.linkeddata.es/def/occupancy-profile#TurnOff
:TurnOff rdf:type owl:NamedIndividual ,
                  :InteractionConcept .


###  http://bimerr.iot.linkeddata.es/def/occupancy-profile#TurnOn
:TurnOn rdf:type owl:NamedIndividual ,
                 :InteractionConcept .


###  http://bimerr.iot.linkeddata.es/def/occupancy-profile#Winter
:Winter rdf:type owl:NamedIndividual ,
                 :Season .


###  http://bimerr.iot.linkeddata.es/def/occupancy-profile#ZoneOnOff
:ZoneOnOff rdf:type owl:NamedIndividual ,
                    :OperationalModeConcept .


###  http://www.w3.org/2006/time#Friday
<http://www.w3.org/2006/time#Friday> rdf:type owl:NamedIndividual ,
                                              <http://www.w3.org/2006/time#DayOfWeek> .


###  http://www.w3.org/2006/time#Monday
<http://www.w3.org/2006/time#Monday> rdf:type owl:NamedIndividual ,
                                              <http://www.w3.org/2006/time#DayOfWeek> .


###  http://www.w3.org/2006/time#Saturday
<http://www.w3.org/2006/time#Saturday> rdf:type owl:NamedIndividual ,
                                                <http://www.w3.org/2006/time#DayOfWeek> .


###  http://www.w3.org/2006/time#Sunday
<http://www.w3.org/2006/time#Sunday> rdf:type owl:NamedIndividual ,
                                              <http://www.w3.org/2006/time#DayOfWeek> .


###  http://www.w3.org/2006/time#Thursday
<http://www.w3.org/2006/time#Thursday> rdf:type owl:NamedIndividual ,
                                                <http://www.w3.org/2006/time#DayOfWeek> .


###  http://www.w3.org/2006/time#Tuesday
<http://www.w3.org/2006/time#Tuesday> rdf:type owl:NamedIndividual ,
                                               <http://www.w3.org/2006/time#DayOfWeek> .


###  http://www.w3.org/2006/time#Wednesday
<http://www.w3.org/2006/time#Wednesday> rdf:type owl:NamedIndividual ,
                                                 <http://www.w3.org/2006/time#DayOfWeek> .


#################################################################
#    Annotations
#################################################################

:Inaction rdfs:comment "The Inaction class represents the decision of an occupant to not act and remain uncomfortable within a space."@en ;
          rdfs:label "Inaction"@en .


#################################################################
#    General axioms
#################################################################

[ rdf:type owl:AllDisjointClasses ;
  owl:members ( :AccousticNeed
                :IAQNeed
                :ThermalNeed
                :VisualNeed
              )
] .


[ rdf:type owl:AllDisjointClasses ;
  owl:members ( :ConstantValueFormula
                :LinearFormula
                :LogitFormula
                :QuadraticFormula
                :WeibullFormula
              )
] .


[ rdf:type owl:AllDifferent ;
  owl:distinctMembers ( :ASHRAEAdaptiveComfort
                        :ASHRAEComfortEnvelop
                        :ISOAdaptiveComfort
                      )
] .


###  Generated by the OWL API (version 5.1.11) https://github.com/owlcs/owlapi/
